# Example 1
$|\psi\rangle=\frac{1}{\sqrt{3}}|00\rangle+\frac{1}{\sqrt{3}}|01\rangle+\frac{1}{\sqrt{6}}|10\rangle+\frac{1}{\sqrt{6}}|11\rangle$
## Case 1:
The 1st Qubit is 0
P(0) = $\frac{1}{3}+\frac{1}{3}=\frac{2}{3}$
On measurement, the state will collapse into 
$|\psi\rangle = \frac{1}{\sqrt{3}}|00\rangle+\frac{1}{\sqrt{3}}|01\rangle$
$|\psi'| =\sqrt{\frac{1}{3}+\frac{1}{3}}=\sqrt{\frac{2}{3}}$
$|\psi'\rangle=$ $\frac{\frac{1}{\sqrt{3}}|00\rangle +\frac{1}{\sqrt{3}}|01\rangle }{\sqrt{\frac{2}{3}}}$ = $\frac{1}{\sqrt{2}}(|00\rangle+|01\rangle)$ =  

Now measure the $2^{nd}$ qubit
P($2^{nd}$ qubit is 0) = $\frac{1}{2}$  
P($2^{nd}$ qubit is 1) = $\frac{1}{2}$  

On measurement, the state will collapse into $|00\rangle$ and  $|01\rangle$
## Case 2:
The 1st Qubit is 1
P(1) = $\frac{1}{6}+\frac{1}{6}=\frac{1}{3}$
On measurement, the state will collapse into 
$|\psi\rangle = \frac{1}{\sqrt{6}}|10\rangle+\frac{1}{\sqrt{6}}|11\rangle$
$|\psi'| =\sqrt{\frac{1}{6}+\frac{1}{6}}=\sqrt{\frac{1}{3}}$
$|\psi'\rangle=$ $\frac{\frac{1}{\sqrt{6}}|10\rangle +\frac{1}{\sqrt{6}}|11\rangle }{\sqrt{\frac{1}{3}}}$ = $\frac{1}{\sqrt{2}}(|10\rangle+|11\rangle)$ =  

Now measure the $2^{nd}$ qubit
P($2^{nd}$ qubit is 0) = $\frac{1}{2}$  
P($2^{nd}$ qubit is 1) = $\frac{1}{2}$  

On measurement, the state will collapse into $|10\rangle$ and  $|11\rangle$

# Example 2
$|\psi\rangle=\frac{1}{3}|00\rangle+\frac{2}{3}|10\rangle-\frac{2}{3}|11\rangle$
## Case 1:
The 1st Qubit is 0
P(0) = $\frac{1}{9}$
On measurement, the state will collapse into 
$|\psi\rangle = \frac{1}{\sqrt{3}}|00\rangle$
$|\psi'| =\sqrt{\frac{1}{3}}$
$|\psi\rangle=$ $|00\rangle$

Now measure the $2^{nd}$ qubit
P($2^{nd}$ qubit is 0) = $1$  
P($2^{nd}$ qubit is 1) = $0$  

On measurement, the state will collapse into $|00\rangle$ and  $|01\rangle$
## Case 2:
The 1st Qubit is 1
P(1) = $\frac{4}{9}+\frac{4}{9}=\frac{8}{9}$
On measurement, the state will collapse into 
$|\psi\rangle = \frac{2}{3}|10\rangle-\frac{2}{3}|11\rangle$
$|\psi'| =\sqrt{\frac{4}{9}+\frac{4}{9}}=\sqrt{\frac{8}{9}}$= $2\frac{\sqrt{2}}{3}$
$|\psi\rangle=$ $\frac{\frac{2}{3}|10\rangle -\frac{2}{3}|11\rangle }{2\frac{\sqrt{2}}{3}}$ = $\frac{1}{\sqrt{2}}(|10\rangle-|11\rangle)$ =  

Now measure the $2^{nd}$ qubit
P($2^{nd}$ qubit is 0) = $\frac{1}{2}$  
P($2^{nd}$ qubit is 1) = $\frac{1}{2}$  

On measurement, the state will collapse into $|10\rangle$ and  $|11\rangle$